+++
title = "Project Euler 28: Number Spiral Diagonals"
author = ["Gautam Manohar"]
description = "My solution to problem 28 of Project Euler."
date = 2018-06-13
tags = ["primes", "math"]
categories = ["euler"]
draft = false
+++

## Problem Statement {#problem-statement}

Starting with the number 1 and moving to the right in a clockwise direction, a
5-by-5 spiral is formed:

{{< figure src="/img/euler/28-spiral.png" caption="Figure 1: A 5-by-5 number spiral. The diagonal entries are bolded." width="250px" >}}

It can be verified that the sum of the numbers on the diagonals is 101. What is
the sum of the numbers on the diagonals in an \\(N \times N\\) spiral (\\(N\\) odd)?
Report your answer modulo \\(10^9 + 7\\).


## My Algorithm {#my-algorithm}

We can think of the spiral as being made up of a central 1 surrounded by \\(n\\)
rings of side length \\(2n+1\\), where \\(n = \frac{N - 1}{2}\\). Let us derive a
formula for the sum of the numbers in the corners of each ring---these make up
the diagonals of the spiral. The number in the top-right corner of the $n$-th
ring is \\((2n+1)^2\\), the area of the ring. Going counter-clockwise, the number
decreases by one less than the side length, or \\(2n+1-1=2n\\), each time. And so
the $n$-th ring has corner sum

\begin{equation}
4(2n+1)^2 - 6(2n) = 16n^2 + 4n + 4.
\end{equation}

To find the sum of the corners of all rings, we can use the formula for the sum
of the first \\(n\\) natural numbers

\begin{equation}
\sum\_{i=0}^n i = \frac{n(n+1)}{2}
\end{equation}

and their squares:

\begin{equation}
\sum\_{i=0}^n i^2 = \frac{n(n+1)(2n+1)}{6}.
\end{equation}

To get the sum of the diagonals, we just add 1 to the sum of the corners, to
account for the central 1. And so our desired answer \\(S\\) is

\begin{equation}
\begin{split}
S &= 1 + \sum\_{i=0}^{\frac{N-1}{2}} (16n^2 + 4n + 4) \\\\\\
&= 1 + 16\cdot\frac{\frac{N-1}{2}\left(\frac{N-1}{2} + 1\right)\left(2\cdot\frac{N-1}{2} + 1\right)}{6} + 4\cdot\frac{\frac{N-1}{2}\left(\frac{N-1}{2}+1\right)}{2} + 4\frac{N-1}{2} \\\\\\
&= 1 + 4\cdot\frac{(N-1)(N - 1 + 2)(N - 1 + 1)}{6} + \frac{(N-1)(N-1+2)}{2} + 2(N-1) \\\\\\
&= 1 + \frac{2N(N-1)(N+1)}{3} + \frac{(N-1)(N+1)}{2} + 2(N-1) \\\\\\
&= \frac{4N(N-1)(N+1) + 3(N-1)(N+1) + 12(N-1) + 6}{6} \\\\\\
&= \frac{4N^3 + 3N^2 + 8N - 9}{6}.
\end{split}
\end{equation}

We report our answer modulo \\(10^9 + 7\\). Because there is a division by 6 in our
answer, we must use the multiplicative modular inverse of 6 modulo \\(10^9 + 7\\),
which we find in \\(O(\log P)\\) time. And so our solution has time complexity
\\(O(1)\\).