+++
title = "Project Euler 65: Convergents of $e$"
author = ["Gautam Manohar"]
description = "My solution to problem 65 of Project Euler."
date = 2018-07-16
tags = ["proof", "continued-fractions"]
categories = ["euler", "math"]
draft = false
shorttitle = "Project Euler 65: Convergents of e"
+++

## Problem Statement {#problem-statement}

The constant \\(e\\) can be written as the infinite continued fraction
\\([2;1,2,1,\,1,4,1,\,1,6,1,\ldots,1,2k,\ldots]\\). Find the sum of the digits in
the $N$-th convergent of the continued fraction expansion for \\(e\\).


## A Recurrence Relation {#a-recurrence-relation}

We will show the following theorem. Let the the $n$-th convergent of a continued
fraction \\([a\_0;a\_1,a\_2,\ldots]\\) be \\(\frac{P\_n}{Q\_n}\\). Then the $(n+1)$-th
convergent is

\begin{equation}
\frac{a\_{n+1}P\_n + P\_{n-1}}{a\_{n+1}Q\_{n} + Q\_{n-1}}.
\end{equation}

We use induction. Because the 0-th convergent is \\(a\_0\\), we define \\(P\_0 = a\_0,
Q\_0 = 1\\). Then the first convergent is

\begin{equation}
a\_0 + \frac{1}{a\_1} = \frac{a\_0a\_1 + 1}{a\_1},
\end{equation}

so \\(P\_1 = a\_0a\_1 + 1, Q\_1 = a\_1\\). As a base case, we show that the formula holds
for \\(n = 2\\):

\begin{equation}
\begin{split}
a\_0 + \frac{1}{a\_1 + \frac{1}{a\_2}} &= a\_0 + \frac{a\_2}{a\_1a\_2 + 1} \\\\\\
&= \frac{a\_0a\_1a\_2 + a\_0 + a\_2}{a\_1a\_2 + 1} \\\\\\
&= \frac{a\_2(a\_0a\_1 + 1) + a\_0}{a\_2a\_1 + 1} \\\\\\
&= \frac{a\_2P\_1 + P\_0}{a\_2Q\_1 + Q\_0}.
\end{split}
\end{equation}

Now suppose inductively that

\begin{equation}
P\_{n} = a\_{n}P\_{n-1} + P\_{n-2}, Q\_{n} = a\_nQ\_{n-1} + Q\_{n-2}.
\end{equation}

The $n$-th convergent is

\begin{equation}
\frac{P\_n}{Q\_n} = a\_1 + \cfrac{1}{a\_2 + \cfrac{1}{\begin{array}{ccc}a\_{3} + & & \\ & \ddots & \\ & & + \cfrac{1}{a\_{n-1} + \cfrac{1}{a\_{n}}}\end{array}}}
\label{n-conv}
\end{equation}

Turning \eqref{n-conv} into the $(n+1)$-th convergent involves replacing \\(a\_n\\)
with \\(a\_n + \frac{1}{a\_{n+1}}\\). Using the recursive formula, this gives

\begin{equation}
\begin{split}
\frac{P\_{n+1}}{Q\_{n+1}} &= \frac{\frac{P\_{n-1}}{a\_{n+1}} + a\_nP\_{n-1} + P\_{n-2}}{\frac{Q\_{n-1}}{a\_{n+1}} + a\_nQ\_{n-1} + Q\_{n-2}} \\\\\\
&= \frac{\frac{P\_{n-1}}{a\_{n+1}} + P\_n}{\frac{Q\_{n-1}}{a\_{n+1}} + Q\_n} \\\\\\
&= \frac{a\_{n+1}P\_n + P\_{n-1}}{a\_{n+1}Q\_{n} + Q\_{n-1}},
\end{split}
\end{equation}

which proves the theorem.


## My Algorithm {#my-algorithm}

Let the $n$-th coefficient in the continued fraction expansion for \\(e\\) be \\(a\_n\\).
Then \\(a\_0 = 2\\). From then on, \\(a\_1 = a\_3 = 1\\), and \\(a\_2 = 2\\). In particular,
\\(a\_n = 1\\) if \\(n\\) is congruent to 0 or 1 mod 3 (unless \\(n = 0\\)). And so

\begin{equation}
a\_n =
\begin{cases}
2 &n = 0, \\\\\\
2\left(\lfloor\frac{n}{3}\rfloor + 1\right) &n \equiv 2 \pmod 3, \\\\\\
1 &\text{otherwise}.
\end{cases}
\end{equation}

Using this and our theorem, we iteratively calculate the numerator of the $N$-th
convergent by

\begin{equation}
P\_n = a\_nP\_{n-1} + P\_{n-2}.
\end{equation}

We cache the previous two convergents at each step. Finally, we take the digit
sum. Our solution has time complexity \\(O(N)\\).